src/Dafny/oldmem.dfy
@@ -1,0 +1,96 @@
+include "types.dfy"
+
+module memory {
+
+import opened types
+
+// TEMPORARY
+datatype ptr = ptr(bid:nat, offset:nat)
+
+// Each cell of memory is occupied by either data, a pointer, or uninitialized
+// data
+datatype MemCell = mb(size:nat, data:byte) |
+                   mptr(block:nat, offset:nat, index:nat) |
+				   muninit()
+				   
+// Memory is composed of a bunch of blocks, each block being a list of memory
+// cells that all start uninitialized
+type Block = seq<MemCell>
+type MemMap = map<nat, Block>
+datatype MemState = MemState(mem:MemMap, nextBlock:nat)
+
+// A newly-initialized block should start out uninitialized, meaning all its
+// members are muninit
+predicate {:opaque} IsUninit(b:Block) {
+	forall offset | 0 <= offset < |b| :: b[offset].muninit?
+}
+
+function UninitBlock(size:nat) : (b:Block)
+	ensures IsUninit(b)
+	ensures |b| == size
+	decreases size
+{
+	reveal_IsUninit();
+	if size == 0 then []
+	else UninitBlock(size - 1) + [muninit()]
+}
+
+// Pointers and block indices can be valid/invalid depending on whether the
+// location exists in memory
+predicate IsValidBlock(s:MemState, bid:nat) {
+	bid in s.mem
+}
+
+predicate IsValidPtr(s:MemState, p:ptr) {
+	&& p.bid in s.mem
+	&& p.offset < |s.mem[p.bid]|
+}
+
+// On initialization, the memory state is empty and contains no blocks
+predicate MemInit(s:MemState) {
+	&& |s.mem| == 0
+	&& s.nextBlock == 0
+}
+
+// Need to check every step to make sure memory is still valid
+predicate MemValid(s:MemState) {
+	forall bid | bid in s.mem :: bid < s.nextBlock
+}
+
+// When a new block is allocated, all the previous blocks should remain the same,
+// and an unininitialized block of the appropriate size should be added with block
+// nextBlock
+predicate Alloc(s:MemState, s':MemState, bid:nat, size:nat) {
+	&& bid == s.nextBlock
+	&& s'.nextBlock == s.nextBlock + 1
+	&& s'.mem == s.mem[s.nextBlock := UninitBlock(size)]
+}
+
+// Blocks can be freed as well, in which case it is simply removed from the map
+predicate Free(s:MemState, s':MemState, bid:nat)
+	requires IsValidBlock(s, bid)
+{
+	&& s'.nextBlock == s.nextBlock
+	&& bid !in s'.mem
+	&& s.mem == s'.mem[bid:= s.mem[bid]]
+}
+
+// TODO: Support reading and writing more than one byte at a time
+predicate Load(s:MemState, s':MemState, p:ptr, val:byte)
+	requires IsValidPtr(s, p)
+{
+	var cell := s.mem[p.bid][p.offset];
+	&& s' == s
+	&& cell.mb?
+	&& cell.data == val
+}	
+
+// TODO: Support reading and writing more than one byte at a time
+predicate Store(s:MemState, s':MemState, p:ptr, val:byte)
+	requires IsValidPtr(s, p)
+{
+	&& s'.nextBlock == s.nextBlock
+	&& s'.mem == s.mem[p.bid := s.mem[p.bid][p.offset := mb(1, val)]]
+}
+
+}
